First attempt to define and type fixpoint combinator

src/Language/PlutusIR/Transform/LetRec.v
@@ -1,7 +1,115 @@
 From PlutusCert Require Import
   Language.PlutusIR
+  Semantics.Static
+  Semantics.Static.Implementations.Named
+  Semantics.Static.Weakening
   .
 Import NamedTerm.
 
-Polymorphic Inductive LetTermsRec : Term -> Term -> Type := .
+From Coq Require Import
+  Strings.String.
 
+Open Scope string_scope.
+
+(*
+T : K
+F : (K => * ) => (K => * )
+---------
+ifix F T : *
+
+
+*)
+
+
+(* Convenience: type-level non-recursive let *)
+Definition Ty_Let var k ty_bound ty_body : Ty :=
+  Ty_App (Ty_Lam var k ty_body) (ty_bound).
+
+Definition k_star_star := (Kind_Arrow Kind_Base Kind_Base).
+Definition ty_id := Ty_Lam "X" Kind_Base (Ty_Var "X").
+
+
+
+(* Encode the Z combinator *)
+
+(* Type to instantiate IFix for regular fixpoint
+   combinator. "F" in IFix F T, this fixes
+   the kind K of T to be * -> *
+*)
+Definition Fix_0_inst : Ty :=
+  (Ty_Lam "Rec" (Kind_Arrow k_star_star Kind_Base)
+    (Ty_Lam "F" (k_star_star)
+      (Ty_App (Ty_Var "F")
+        (Ty_App (Ty_Var "Rec") (Ty_Var "F"))
+      )
+    )
+  ).
+
+Definition Fix_0 (t : Ty) : Ty :=
+  Ty_IFix Fix_0_inst t
+.
+
+Lemma Fix_0_well_kinded : forall t,
+  emptyContext |-* t : k_star_star ->
+  emptyContext |-* (Fix_0 t) : Kind_Base.
+Proof. repeat econstructor. assumption. Qed.
+
+(* wrap specialized to Fix0_inst *)
+Definition wrap_0 (ty : Ty) (t : Term) : Term :=
+  IWrap Fix_0_inst ty t.
+
+(* Instantiation for the second argument of IFix
+   (first argument of Fix_0)
+   This has to be of kind * -> * (not as a meta-construction that
+   accepts types, otherwise it cannot be used as argument of wrap or IFix
+*)
+Definition Self_inst :=
+  (Ty_Lam "A" Kind_Base
+    ( Ty_Lam "Rec" Kind_Base
+        ( Ty_Fun (Ty_Var "Rec") (Ty_Var "A") )
+    )
+  ).
+
+Definition Self :=
+  (Ty_Lam "A" Kind_Base
+    (Fix_0 (Ty_App Self_inst (Ty_Var "A"))
+    )
+  ).
+
+Lemma Self_well_kinded : emptyContext |-* Self : k_star_star.
+Proof. repeat econstructor. Qed.
+
+Definition self_type :=
+  (
+    Ty_Forall "A" Kind_Base
+    (
+      (Ty_Fun
+        (Ty_Fun
+          (Ty_App Self (Ty_Var "A"))
+          (Ty_Var "A")
+        )
+        (Ty_App Self (Ty_Var "A")
+        )
+      )
+    )
+  ).
+
+Definition self :=
+  TyAbs "A" Kind_Base
+    ( LamAbs "f" (Ty_Fun (Ty_App Self (Ty_Var "A")) (Ty_Var "A"))
+        (wrap_0 Self_inst (Var "f"))
+    ).
+
+
+Definition beta := beta_reduce _ _ substituteT.
+Eval cbv in beta self_type.
+Lemma self_well_typed :
+  emptyContext |-+ self : (beta self_type).
+Proof.
+  unfold self_type, self, Self, wrap_0, Fix_0.
+  unfold Self_inst.
+  simpl.
+  repeat econstructor.
+  (* we are stuck, since the type has to be normalized *)
+  Fail apply T_LamAbs.
+Abort.
